Add semantics to base ring for TensorGraph using semantics for tensorlists

theories/GraphCore/TensorGraph.v
@@ -1,90 +1,195 @@
-Require Import Tensor.
-From stdpp Require Import gmap. 
-From stdpp Require Import list.
-Require Import TensorExprDBSyntax.
-Require Import ZXCore.
 From QuantumLib Require Import Complex.
+Require Import Tensor.
+From stdpp Require Import list fin_maps.
+From stdpp Require Import pmap gmap. 
+Require Import TensorExprDBSyntax TensorExprDBSemantics.
+Require Import ZXCore.
+Require ZifyBool.
 
-Definition TensorMap {R : Type} (A : Type) := 
+Definition enumerate {A} (l : list A) : list (nat * A) :=
+  imap pair l.
+
+Definition bcons (b : bool) (p : positive) : positive :=
+  match b with 
+  | true => xI p
+  | false => xO p
+  end.
+
+#[global] 
+Program Instance Op_bcons : ZifyClasses.BinOp 
+  (T1:=bool) bcons := {
+  TBOp b p := (2 * p + Z.b2z b)%Z;
+}.
+Next Obligation.
+  cbn.
+  intros [] ?; cbn; lia.
+Qed.
+
+Add Zify BinOp Op_bcons.
+
+#[export] Instance bcons_inj2 : Inj2 (=) (=) (=) bcons.
+Proof.
+  hnf.
+  lia.
+Qed.
+
+Section TensorGraph.
+
+Context {R : Type} {A : Type}.
+
+Definition TensorMap := 
   gmap nat (DimensionlessTensor (R:=R) A).
 
 Definition EdgeSet := list (nat * nat).
 
-Definition TensorGraph {R} {A} := 
-  ((TensorMap (R:=R) A) * EdgeSet)%type.
+Definition TensorGraph := 
+  (TensorMap * EdgeSet)%type.
 
-Definition is_key {R} {A} (n : nat) 
-  (tg : TensorGraph (R:=R) (A:=A)) : bool :=
-  match (lookup n (fst tg)) with
-  | Some _ => true
-  | None => false
-  end.
+Definition is_key (tg : TensorGraph) (n : nat) : Prop :=
+  is_Some (tg.1 !! n).
 
-Definition is_input {R} {A} (nm : nat * nat)
-  (tg : TensorGraph (R:=R) (A:=A)) : bool :=
-  is_key (fst nm) tg.
+Definition is_input (tg : TensorGraph) (nm : nat * nat) : Prop :=
+  is_key tg (fst nm).
 
-Definition is_output {R} {A} (nm : nat * nat)
-  (tg : TensorGraph (R:=R) (A:=A)) : bool :=
-  is_key (snd nm) tg.
+Definition is_output (tg : TensorGraph) (nm : nat * nat) : Prop :=
+  is_key tg (snd nm).
 
-Definition count_inputs
-  {R} {A} (tg : TensorGraph (R:=R) (A:=A)) : nat := 
-  length (filter (fun x => is_input x tg) (snd tg)).
+Definition count_inputs (tg : TensorGraph) : nat := 
+  length (filter (is_input tg) (snd tg)).
 
-Definition count_outputs
-  {R} {A} (tg : TensorGraph (R:=R) (A:=A)) : nat := 
-  length (filter (fun x => is_output x tg) (snd tg)).
+Definition count_outputs (tg : TensorGraph) : nat := 
+  length (filter (is_output tg) (snd tg)).
 
-Definition graph_semantics {R} {A} 
-  (tg : TensorGraph (R:=R) (A:=A)) : tensorlist :=
+Definition inputs (tg : TensorGraph) : gset nat :=
+  filter (fun k => ~ is_key tg k) $ 
+    list_to_set tg.2.*1.
 
-  let nodes := map_to_list (fst tg) in
-  let edges := snd tg in
+Definition outputs (tg : TensorGraph) : gset nat :=
+  filter (fun k => ~ is_key tg k) $ 
+    list_to_set tg.2.*2.
 
-  let is_internal e := is_key (fst e) tg && is_key (snd e) tg in
-  let not_internal e := negb (is_internal e) in
 
-  let internal_edges := filter is_internal edges in
-  let external_edges := filter not_internal edges in
+Definition is_internal tg (e : nat * nat) := 
+  is_key tg (fst e) /\ is_key tg (snd e).
 
-  let index_list := imap (fun idx e => (idx, e)) in
+Definition not_internal tg (e : nat * nat) :=
+  ~ is_internal tg e.
 
-  let i_internal_edges := index_list internal_edges in
-  let i_external_edges := index_list external_edges in
 
-  let mk_ivar (e : nat * (nat * nat)) :=
-    rel (Pos.of_succ_nat (fst e)) in
+Definition internal_edges tg := 
+  filter (is_internal tg) tg.2.
 
-  let offset := (Pos.of_succ_nat (length internal_edges)) in 
+Definition external_edges tg :=
+  filter (not_internal tg) tg.2.
 
-  let mk_ovar (e : nat * (nat * nat)) :=
-    loc (Pos.of_succ_nat (fst e) + offset) in
+Definition i_internal_edges tg := 
+  enumerate (internal_edges tg).
 
-  let mk_node (ndt : nat * DimensionlessTensor (R:=R) A) :=
-    let n := fst ndt in
+Definition i_external_edges tg :=
+  enumerate (external_edges tg).
+
+Definition mk_internal_var (e : nat * (nat * nat)) :=
+  rel (Pos.of_succ_nat (fst e)).
+
+Definition mk_external_var (is_output : bool) (e : nat * (nat * nat)) :=
+  loc (bcons is_output (Pos.of_succ_nat (if is_output then e.2.2 else e.2.1))).
+
+Definition mk_node (tg : TensorGraph)
+  (n : nat) : Idx * list var * list var :=
     let is_input e := snd (snd e) =? n in
     let is_output e := fst (snd e) =? n in
-    let i_internal_inputs  := filter is_input i_internal_edges in
-    let i_internal_outputs := filter is_output i_internal_edges in
-    let i_external_inputs  := filter is_input i_external_edges in
-    let i_external_outputs := filter is_output i_external_edges in
+    let i_internal_inputs  := filter is_input (i_internal_edges tg) in
+    let i_internal_outputs := filter is_output (i_internal_edges tg) in
+    let i_external_inputs  := filter is_input (i_external_edges tg) in
+    let i_external_outputs := filter is_output (i_external_edges tg) in
     (Pos.of_succ_nat n, 
-      (mk_ivar <$> i_internal_inputs) ++ (mk_ovar <$> i_external_inputs), (mk_ivar <$> i_internal_outputs) ++ (mk_ovar <$> i_external_outputs)) in
+      (mk_internal_var <$> i_internal_inputs) ++ 
+        (mk_external_var false <$> i_external_inputs), 
+      (mk_internal_var <$> i_internal_outputs) ++ 
+        (mk_external_var true <$> i_external_outputs)).
 
-  let body := mk_node <$> nodes in
 
-  mk_tl (const 0%nat <$> internal_edges) body.
 
-Definition add_vertex {R} {A} (n : nat) (t : DimensionlessTensor (R:=R) A) 
-  (tg : TensorGraph  (R:=R) (A:=A)) : TensorGraph (R:=R) (A:=A) :=
+
+Definition add_vertex (n : nat) (t : DimensionlessTensor (R:=R) A) 
+  (tg : TensorGraph) : TensorGraph:=
   (<[n := t]> (fst tg), snd tg).
 
-Definition add_edge {R} {A} (e : nat * nat) 
-  (tg : TensorGraph (R:=R) (A:=A)) : TensorGraph (R:=R) (A:=A) :=
+Definition add_edge (e : nat * nat) 
+  (tg : TensorGraph) : TensorGraph :=
   (fst tg, e :: snd tg).
 
-Definition empty_graph {R} {A} : TensorGraph (R:=R) (A:=A) := (∅, []).
+Definition empty_graph : TensorGraph := (∅, []).
+
+
+
+
+Definition graph_tensorlist_semantics (tg : TensorGraph) : tensorlist :=
+  mk_tl (const 0%nat <$> internal_edges tg) 
+    (mk_node tg <$> (map_to_list (fst tg)).*1).
+
+Definition graph_V : nat -> Type := fun _ => A.
+Definition graph_Vsum `{Summable A} : forall k, Summable (graph_V k) 
+  := fun _ => _.
+
+(* Combine input and output maps to get the local variable map *)
+Definition graph_ml (minput : gmap nat A) (moutput : gmap nat A) : 
+  Pmap (Vval graph_V) :=
+  @mk_Vval graph_V 0 <$> (kmap (bcons false ∘ Pos.of_succ_nat) minput ∪ 
+      kmap (bcons true ∘ Pos.of_succ_nat) moutput).
+
+Fixpoint graph_tensor_to_V_n_args_aux {n} : forall (t : vec A n -> R),
+  V_n_args graph_V (replicate n 0) R :=
+  match n with
+  | O => fun t => t [#]
+  | S n' => fun t => 
+    fun a => graph_tensor_to_V_n_args_aux (t ∘ vcons a)
+  end.
+
+Definition graph_tensor_to_V_n_args {n m} (t : vec A n -> vec A m -> R) :=
+  graph_tensor_to_V_n_args_aux (uncurry t ∘ Vector.splitat n).
+
+Definition graph_mabs (tg : TensorGraph) : Pmap (@Vfunc R graph_V) :=
+  kmap (Pos.of_succ_nat) $ map_imap (fun n (dt : DimensionlessTensor A) => 
+    let node := mk_node tg n in 
+    let inarity := length node.1.2 in 
+    let outarity := length node.2 in 
+    Some $ mk_Vfunc graph_V (replicate (inarity + outarity) 0)
+      (graph_tensor_to_V_n_args (dt inarity outarity))
+    ) tg.1.
+
+Definition graph_map_semantics `{SR : SemiRing R rO rI radd rmul req} `{!Summable A} 
+  (tg : TensorGraph) 
+  (minput : gmap nat A) (moutput : gmap nat A) : R :=
+  tl_total_semantics (SR:=SR) graph_V (Vsum:=graph_Vsum)
+    (graph_mabs tg)
+    ∅
+    (graph_ml minput moutput)
+    (graph_tensorlist_semantics tg).
+
+Definition graph_insize (tg : TensorGraph) : nat := size (inputs tg).
+Definition graph_outsize (tg : TensorGraph) : nat := size (outputs tg).
+
+From stdpp Require Import sorting.
+
+Definition sorted_inputs (tg : TensorGraph) : list nat :=
+  merge_sort le $ elements (inputs tg).
+
+Definition sorted_outputs (tg : TensorGraph) : list nat :=
+  merge_sort le $ elements (outputs tg).
+
+
+Definition graph_list_semantics `{SR : SemiRing R rO rI radd rmul req} `{!Summable A} 
+  (tg : TensorGraph) (ins : list A) (outs : list A) : R :=
+  graph_map_semantics tg 
+    (list_to_map $ zip (sorted_inputs tg) ins)
+    (list_to_map $ zip (sorted_outputs tg) outs).
+
+Definition graph_vector_semantics `{SR : SemiRing R rO rI radd rmul req} `{!Summable A} 
+  (tg : TensorGraph) (ins : vec A (graph_insize tg)) (outs : vec A (graph_outsize tg)) : R :=
+  graph_list_semantics tg (vec_to_list ins) (vec_to_list outs).
+
+End TensorGraph.
 
 Declare Scope graph_scope.
 Delimit Scope graph_scope with graph.
@@ -102,4 +207,80 @@ Definition example_graph : TensorGraph (R:=C) (A:=bool) :=
      +[ 3 := (fun n m => @zsp n m 0) ]
      +{ (1,2) ; (1,3) ; (1,2) ; (1,3) ; (1,4) }.
 
-Compute graph_semantics example_graph.
+
+Definition example_graph' : TensorGraph (R:=C) (A:=bool) := 
+  ∅G +[ 1 := (fun n m => @zsp n m 0) ]
+     +[ 3 := (fun n m => @zsp n m 0) ]
+     +{ (1,2) ; (1,3) ; (3,4) }.
+
+Compute graph_tensorlist_semantics example_graph.
+
+Compute elements $ inputs example_graph.
+
+Compute elements $ outputs example_graph.
+
+Compute graph_tensorlist_semantics example_graph'.
+
+Compute elements $ inputs example_graph'.
+
+Compute elements $ outputs example_graph'.
+
+
+(* 
+From VyZX Require Import CoreData.
+
+Open Scope ZX_scope.
+
+Open Scope nat_scope.
+
+Example example_graph'_map_semantics : forall b b',
+  graph_map_semantics example_graph' 
+    ∅ {[2:=b; 4:=b']} = 
+  ⟦ Z 0 2 0 ⟷ (— ↕ Z 1 1 0) ⟧
+    (Bits.funbool_to_nat 2 ([b;b'] !!!.)) O.
+Proof.
+  cbn -[graph_map_semantics].
+  unfold kron.
+  cbn -[graph_map_semantics].
+  intros [] []; cbn -[graph_map_semantics]; (etransitivity; 
+    [unfold example_graph'; 
+      remember @zsp as zsp' eqn:Hzsp; 
+      vm_compute|Csimpl; reflexivity]);
+  subst zsp'; cbn -[Cexp]; 
+  change R0 with 0%R; rewrite ?Cexp_0; lca.
+Qed.
+
+Example example_graph'_list_semantics : forall b b',
+  graph_list_semantics example_graph' 
+    [] [b; b'] = 
+  ⟦ Z 0 2 0 ⟷ (— ↕ Z 1 1 0) ⟧
+    (Bits.funbool_to_nat 2 ([b;b'] !!!.)) O.
+Proof.
+  cbn -[graph_list_semantics].
+  unfold kron.
+  cbn -[graph_list_semantics].
+  intros [] []; cbn -[graph_list_semantics]; (etransitivity; 
+    [unfold example_graph'; 
+      remember @zsp as zsp' eqn:Hzsp; 
+      vm_compute|Csimpl; reflexivity]);
+  subst zsp'; cbn -[Cexp]; 
+  change R0 with 0%R; rewrite ?Cexp_0; lca.
+Qed.
+
+Example example_graph'_vector_semantics : forall b b',
+  graph_vector_semantics example_graph' 
+    [# ] [# b; b'] = 
+  ⟦ Z 0 2 0 ⟷ (— ↕ Z 1 1 0) ⟧
+    (Bits.funbool_to_nat 2 ([b;b'] !!!.)) O.
+Proof.
+  cbn -[graph_vector_semantics].
+  unfold kron.
+  cbn -[graph_vector_semantics].
+  intros [] []; cbn -[graph_vector_semantics]; (etransitivity; 
+    [unfold example_graph'; 
+      remember @zsp as zsp' eqn:Hzsp; 
+      vm_compute|Csimpl; reflexivity]);
+  subst zsp'; cbn -[Cexp]; 
+  change R0 with 0%R; rewrite ?Cexp_0; lca.
+Qed.
+ *)
